src/sequential/SeqLiftStep.v
@@ -998,6 +998,7 @@ Proof.
   { i. hexploit sim_promises_get; eauto. i. des. esplits.
     { eapply PRESERVE; eauto. eapply memory_get_ts_le; eauto. }
     { eapply PRESERVE; eauto. refl. }
+    { auto. }
     { i. hexploit GET0; eauto. i. des. esplits; eauto.
       erewrite <- sim_message_max_mon_mapping; eauto.
     }
